src/code/kubernetes_model/apimodel.v
@@ -113,19 +113,12 @@ Definition State__objGetⁱᵐᵖˡ : val :=
     else return: (#interface.nil, ![#boolT] "exists"))).
 
 (* go: api_model.go:76:17 *)
-Definition State__objListⁱᵐᵖˡ : val :=
+Definition State__objListLockedⁱᵐᵖˡ : val :=
   λ: "s" "kind" "namespace",
-    with_defer: (let: "items" := (mem.alloc (type.zero_val #sliceT)) in
+    exception_do (let: "items" := (mem.alloc (type.zero_val #sliceT)) in
     let: "s" := (mem.alloc "s") in
     let: "namespace" := (mem.alloc "namespace") in
     let: "kind" := (mem.alloc "kind") in
-    do:  ((method_call #(ptrT.id sync.Mutex.id) #"Lock"%go (![#ptrT] (struct.field_ref #State #"mu"%go (![#ptrT] "s")))) #());;;
-    do:  (let: "$f" := (method_call #(ptrT.id sync.Mutex.id) #"Unlock"%go (![#ptrT] (struct.field_ref #State #"mu"%go (![#ptrT] "s")))) in
-    "$defer" <-[#funcT] (let: "$oldf" := (![#funcT] "$defer") in
-    (λ: <>,
-      "$f" #();;
-      "$oldf" #()
-      )));;;
     let: "$range" := (![type.mapT #KKey #interfaceT] (struct.field_ref #State #"m"%go (![#ptrT] "s"))) in
     (let: "val" := (mem.alloc (type.zero_val #interfaceT)) in
     let: "key" := (mem.alloc (type.zero_val #KKey)) in
@@ -146,9 +139,27 @@ Definition State__objListⁱᵐᵖˡ : val :=
       else do:  #())));;;
     return: (![#sliceT] "items")).
 
+(* go: api_model.go:87:17 *)
+Definition State__objListⁱᵐᵖˡ : val :=
+  λ: "s" "kind" "namespace",
+    with_defer: (let: "items" := (mem.alloc (type.zero_val #sliceT)) in
+    let: "s" := (mem.alloc "s") in
+    let: "namespace" := (mem.alloc "namespace") in
+    let: "kind" := (mem.alloc "kind") in
+    do:  ((method_call #(ptrT.id sync.Mutex.id) #"Lock"%go (![#ptrT] (struct.field_ref #State #"mu"%go (![#ptrT] "s")))) #());;;
+    do:  (let: "$f" := (method_call #(ptrT.id sync.Mutex.id) #"Unlock"%go (![#ptrT] (struct.field_ref #State #"mu"%go (![#ptrT] "s")))) in
+    "$defer" <-[#funcT] (let: "$oldf" := (![#funcT] "$defer") in
+    (λ: <>,
+      "$f" #();;
+      "$oldf" #()
+      )));;;
+    return: (let: "$a0" := (![#stringT] "kind") in
+     let: "$a1" := (![#stringT] "namespace") in
+     (method_call #(ptrT.id State.id) #"objListLocked"%go (![#ptrT] "s")) "$a0" "$a1")).
+
 Definition filterByLabelSelector : go_string := "kubernetes_model/apimodel.filterByLabelSelector"%go.
 
-(* go: api_model.go:90:6 *)
+(* go: api_model.go:94:6 *)
 Definition filterByLabelSelectorⁱᵐᵖˡ : val :=
   λ: "items" "selector",
     exception_do (let: "selector" := (mem.alloc "selector") in
@@ -181,7 +192,7 @@ Definition filterByLabelSelectorⁱᵐᵖˡ : val :=
       else do:  #())));;;
     return: (![#sliceT] "filtered_items", #interface.nil)).
 
-(* go: api_model.go:104:17 *)
+(* go: api_model.go:108:17 *)
 Definition State__objListBySelectorⁱᵐᵖˡ : val :=
   λ: "s" "kind" "namespace" "selector",
     exception_do (let: "s" := (mem.alloc "s") in
@@ -197,7 +208,7 @@ Definition State__objListBySelectorⁱᵐᵖˡ : val :=
 
 Definition randomSuffix : go_string := "kubernetes_model/apimodel.randomSuffix"%go.
 
-(* go: api_model.go:108:6 *)
+(* go: api_model.go:112:6 *)
 Definition randomSuffixⁱᵐᵖˡ : val :=
   λ: "n",
     exception_do (let: "n" := (mem.alloc "n") in
@@ -222,7 +233,7 @@ Definition randomSuffixⁱᵐᵖˡ : val :=
       do:  ((slice.elem_ref #byteT (![#sliceT] "b") (![#intT] "i")) <-[#byteT] "$r0")));;;
     return: (string.from_bytes (![#sliceT] "b"))).
 
-(* go: api_model.go:118:17 *)
+(* go: api_model.go:122:17 *)
 Definition State__generateNewNameⁱᵐᵖˡ : val :=
   λ: "s" "kind" "namespace" "generateName",
     exception_do (let: "s" := (mem.alloc "s") in
@@ -254,7 +265,7 @@ Definition State__generateNewNameⁱᵐᵖˡ : val :=
       then return: (![#stringT] "name")
       else do:  #())))).
 
-(* go: api_model.go:132:17 *)
+(* go: api_model.go:136:17 *)
 Definition State__generateNewUIDAndUpdateⁱᵐᵖˡ : val :=
   λ: "s" <>,
     exception_do (let: "s" := (mem.alloc "s") in
@@ -282,7 +293,7 @@ Definition State__generateNewUIDAndUpdateⁱᵐᵖˡ : val :=
         return: (![#stringT] "uidStr")
       else do:  #())))).
 
-(* go: api_model.go:143:17 *)
+(* go: api_model.go:147:17 *)
 Definition State__objCreateⁱᵐᵖˡ : val :=
   λ: "s" "kind" "namespace" "obj",
     with_defer: (let: "s" := (mem.alloc "s") in
@@ -381,7 +392,7 @@ Definition State__objCreateⁱᵐᵖˡ : val :=
     return: (let: "$a0" := (![#interfaceT] "objCopy") in
      (func_call #deepCopy) "$a0", #interface.nil)).
 
-(* go: api_model.go:186:17 *)
+(* go: api_model.go:190:17 *)
 Definition State__objUpdateⁱᵐᵖˡ : val :=
   λ: "s" "kind" "namespace" "obj",
     with_defer: (let: "s" := (mem.alloc "s") in
@@ -517,7 +528,7 @@ Definition State__objUpdateⁱᵐᵖˡ : val :=
     return: (let: "$a0" := (![#interfaceT] "objCopy") in
      (func_call #deepCopy) "$a0", #interface.nil)).
 
-(* go: api_model.go:236:17 *)
+(* go: api_model.go:240:17 *)
 Definition State__objDeleteⁱᵐᵖˡ : val :=
   λ: "s" "key",
     with_defer: (let: "s" := (mem.alloc "s") in
@@ -586,7 +597,7 @@ Definition State__objDeleteⁱᵐᵖˡ : val :=
 
 Definition index_of : go_string := "kubernetes_model/apimodel.index_of"%go.
 
-(* go: api_model.go:264:6 *)
+(* go: api_model.go:268:6 *)
 Definition index_ofⁱᵐᵖˡ : val :=
   λ: "indexName" "obj",
     exception_do (let: "obj" := (mem.alloc "obj") in
@@ -616,13 +627,20 @@ Definition index_ofⁱᵐᵖˡ : val :=
 
 (* Returned value must be treated as read-only.
 
-   go: api_model.go:279:17 *)
+   go: api_model.go:283:17 *)
 Definition State__Indexⁱᵐᵖˡ : val :=
   λ: "s" "kind" "indexName" "obj",
-    exception_do (let: "s" := (mem.alloc "s") in
+    with_defer: (let: "s" := (mem.alloc "s") in
     let: "obj" := (mem.alloc "obj") in
     let: "indexName" := (mem.alloc "indexName") in
     let: "kind" := (mem.alloc "kind") in
+    do:  ((method_call #(ptrT.id sync.Mutex.id) #"Lock"%go (![#ptrT] (struct.field_ref #State #"mu"%go (![#ptrT] "s")))) #());;;
+    do:  (let: "$f" := (method_call #(ptrT.id sync.Mutex.id) #"Unlock"%go (![#ptrT] (struct.field_ref #State #"mu"%go (![#ptrT] "s")))) in
+    "$defer" <-[#funcT] (let: "$oldf" := (![#funcT] "$defer") in
+    (λ: <>,
+      "$f" #();;
+      "$oldf" #()
+      )));;;
     let: "err" := (mem.alloc (type.zero_val #error)) in
     let: "indexedValues" := (mem.alloc (type.zero_val #sliceT)) in
     let: ("$ret0", "$ret1") := (let: "$a0" := (![#stringT] "indexName") in
@@ -658,7 +676,7 @@ Definition State__Indexⁱᵐᵖˡ : val :=
     let: "items" := (mem.alloc (type.zero_val #sliceT)) in
     let: "$range" := (let: "$a0" := (![#stringT] "kind") in
     let: "$a1" := #v1.NamespaceAll in
-    (method_call #(ptrT.id State.id) #"objList"%go (![#ptrT] "s")) "$a0" "$a1") in
+    (method_call #(ptrT.id State.id) #"objListLocked"%go (![#ptrT] "s")) "$a0" "$a1") in
     (let: "val" := (mem.alloc (type.zero_val #interfaceT)) in
     slice.for_range #interfaceT "$range" (λ: "$key" "$value",
       do:  ("val" <-[#interfaceT] "$value");;;
@@ -700,18 +718,25 @@ Definition State__Indexⁱᵐᵖˡ : val :=
 
 (* Returned value must be treated as read-only.
 
-   go: api_model.go:311:17 *)
+   go: api_model.go:318:17 *)
 Definition State__ByIndexⁱᵐᵖˡ : val :=
   λ: "s" "kind" "indexName" "indexedValue",
-    exception_do (let: "s" := (mem.alloc "s") in
+    with_defer: (let: "s" := (mem.alloc "s") in
     let: "indexedValue" := (mem.alloc "indexedValue") in
     let: "indexName" := (mem.alloc "indexName") in
     let: "kind" := (mem.alloc "kind") in
+    do:  ((method_call #(ptrT.id sync.Mutex.id) #"Lock"%go (![#ptrT] (struct.field_ref #State #"mu"%go (![#ptrT] "s")))) #());;;
+    do:  (let: "$f" := (method_call #(ptrT.id sync.Mutex.id) #"Unlock"%go (![#ptrT] (struct.field_ref #State #"mu"%go (![#ptrT] "s")))) in
+    "$defer" <-[#funcT] (let: "$oldf" := (![#funcT] "$defer") in
+    (λ: <>,
+      "$f" #();;
+      "$oldf" #()
+      )));;;
     let: "items" := (mem.alloc (type.zero_val #sliceT)) in
     let: "listed" := (mem.alloc (type.zero_val #sliceT)) in
     let: "$r0" := (let: "$a0" := (![#stringT] "kind") in
     let: "$a1" := #v1.NamespaceAll in
-    (method_call #(ptrT.id State.id) #"objList"%go (![#ptrT] "s")) "$a0" "$a1") in
+    (method_call #(ptrT.id State.id) #"objListLocked"%go (![#ptrT] "s")) "$a0" "$a1") in
     do:  ("listed" <-[#sliceT] "$r0");;;
     let: "$range" := (![#sliceT] "listed") in
     (let: "val" := (mem.alloc (type.zero_val #interfaceT)) in
@@ -748,7 +773,7 @@ Definition State__ByIndexⁱᵐᵖˡ : val :=
 
 (* Returned value must be treated as read-only.
 
-   go: api_model.go:330:17 *)
+   go: api_model.go:340:17 *)
 Definition State__PodGetⁱᵐᵖˡ : val :=
   λ: "s" "namespace" "name",
     exception_do (let: "s" := (mem.alloc "s") in
@@ -759,7 +784,7 @@ Definition State__PodGetⁱᵐᵖˡ : val :=
     (method_call #(ptrT.id State.id) #"PodMutGet"%go (![#ptrT] "s")) "$a0" "$a1")) in
     return: ("$ret0", "$ret1")).
 
-(* go: api_model.go:334:17 *)
+(* go: api_model.go:344:17 *)
 Definition State__PodMutGetⁱᵐᵖˡ : val :=
   λ: "s" "namespace" "name",
     exception_do (let: "s" := (mem.alloc "s") in
@@ -809,7 +834,7 @@ Definition State__PodMutGetⁱᵐᵖˡ : val :=
 
 (* Returned value must be treated as read-only.
 
-   go: api_model.go:356:17 *)
+   go: api_model.go:366:17 *)
 Definition State__PodListⁱᵐᵖˡ : val :=
   λ: "s" "namespace" "selector",
     exception_do (let: "s" := (mem.alloc "s") in
@@ -820,7 +845,7 @@ Definition State__PodListⁱᵐᵖˡ : val :=
     (method_call #(ptrT.id State.id) #"PodMutList"%go (![#ptrT] "s")) "$a0" "$a1")) in
     return: ("$ret0", "$ret1")).
 
-(* go: api_model.go:360:17 *)
+(* go: api_model.go:370:17 *)
 Definition State__PodMutListⁱᵐᵖˡ : val :=
   λ: "s" "namespace" "selector",
     exception_do (let: "s" := (mem.alloc "s") in
@@ -868,7 +893,7 @@ Definition State__PodMutListⁱᵐᵖˡ : val :=
       do:  ("pods" <-[#sliceT] "$r0")));;;
     return: (![#sliceT] "pods", #interface.nil)).
 
-(* go: api_model.go:378:17 *)
+(* go: api_model.go:388:17 *)
 Definition State__PodCreateⁱᵐᵖˡ : val :=
   λ: "s" "namespace" "pod",
     exception_do (let: "s" := (mem.alloc "s") in
@@ -901,7 +926,7 @@ Definition State__PodCreateⁱᵐᵖˡ : val :=
     else do:  #());;;
     return: (![#ptrT] "pod", ![#error] "err")).
 
-(* go: api_model.go:393:17 *)
+(* go: api_model.go:403:17 *)
 Definition State__PodUpdateⁱᵐᵖˡ : val :=
   λ: "s" "namespace" "pod",
     exception_do (let: "s" := (mem.alloc "s") in
@@ -934,7 +959,7 @@ Definition State__PodUpdateⁱᵐᵖˡ : val :=
     else do:  #());;;
     return: (![#ptrT] "pod", ![#error] "err")).
 
-(* go: api_model.go:408:17 *)
+(* go: api_model.go:418:17 *)
 Definition State__PodDeleteⁱᵐᵖˡ : val :=
   λ: "s" "namespace" "name",
     exception_do (let: "s" := (mem.alloc "s") in
@@ -955,7 +980,7 @@ Definition State__PodDeleteⁱᵐᵖˡ : val :=
 
 (* Returned value must be treated as read-only.
 
-   go: api_model.go:419:17 *)
+   go: api_model.go:429:17 *)
 Definition State__ReplicaSetGetⁱᵐᵖˡ : val :=
   λ: "s" "namespace" "name",
     exception_do (let: "s" := (mem.alloc "s") in
@@ -966,7 +991,7 @@ Definition State__ReplicaSetGetⁱᵐᵖˡ : val :=
     (method_call #(ptrT.id State.id) #"ReplicaSetMutGet"%go (![#ptrT] "s")) "$a0" "$a1")) in
     return: ("$ret0", "$ret1")).
 
-(* go: api_model.go:423:17 *)
+(* go: api_model.go:433:17 *)
 Definition State__ReplicaSetMutGetⁱᵐᵖˡ : val :=
   λ: "s" "namespace" "name",
     exception_do (let: "s" := (mem.alloc "s") in
@@ -1018,7 +1043,7 @@ Definition vars' : list (go_string * go_type) := [].
 
 Definition functions' : list (go_string * val) := [(NewState, NewStateⁱᵐᵖˡ); (deepCopy, deepCopyⁱᵐᵖˡ); (filterByLabelSelector, filterByLabelSelectorⁱᵐᵖˡ); (randomSuffix, randomSuffixⁱᵐᵖˡ); (index_of, index_ofⁱᵐᵖˡ)].
 
-Definition msets' : list (go_string * (list (go_string * val))) := [(State.id, []); (ptrT.id State.id, [("ByIndex"%go, State__ByIndexⁱᵐᵖˡ); ("Index"%go, State__Indexⁱᵐᵖˡ); ("PodCreate"%go, State__PodCreateⁱᵐᵖˡ); ("PodDelete"%go, State__PodDeleteⁱᵐᵖˡ); ("PodGet"%go, State__PodGetⁱᵐᵖˡ); ("PodList"%go, State__PodListⁱᵐᵖˡ); ("PodMutGet"%go, State__PodMutGetⁱᵐᵖˡ); ("PodMutList"%go, State__PodMutListⁱᵐᵖˡ); ("PodUpdate"%go, State__PodUpdateⁱᵐᵖˡ); ("ReplicaSetGet"%go, State__ReplicaSetGetⁱᵐᵖˡ); ("ReplicaSetMutGet"%go, State__ReplicaSetMutGetⁱᵐᵖˡ); ("generateNewName"%go, State__generateNewNameⁱᵐᵖˡ); ("generateNewUIDAndUpdate"%go, State__generateNewUIDAndUpdateⁱᵐᵖˡ); ("objCreate"%go, State__objCreateⁱᵐᵖˡ); ("objDelete"%go, State__objDeleteⁱᵐᵖˡ); ("objGet"%go, State__objGetⁱᵐᵖˡ); ("objList"%go, State__objListⁱᵐᵖˡ); ("objListBySelector"%go, State__objListBySelectorⁱᵐᵖˡ); ("objUpdate"%go, State__objUpdateⁱᵐᵖˡ)]); (KKey.id, []); (ptrT.id KKey.id, [])].
+Definition msets' : list (go_string * (list (go_string * val))) := [(State.id, []); (ptrT.id State.id, [("ByIndex"%go, State__ByIndexⁱᵐᵖˡ); ("Index"%go, State__Indexⁱᵐᵖˡ); ("PodCreate"%go, State__PodCreateⁱᵐᵖˡ); ("PodDelete"%go, State__PodDeleteⁱᵐᵖˡ); ("PodGet"%go, State__PodGetⁱᵐᵖˡ); ("PodList"%go, State__PodListⁱᵐᵖˡ); ("PodMutGet"%go, State__PodMutGetⁱᵐᵖˡ); ("PodMutList"%go, State__PodMutListⁱᵐᵖˡ); ("PodUpdate"%go, State__PodUpdateⁱᵐᵖˡ); ("ReplicaSetGet"%go, State__ReplicaSetGetⁱᵐᵖˡ); ("ReplicaSetMutGet"%go, State__ReplicaSetMutGetⁱᵐᵖˡ); ("generateNewName"%go, State__generateNewNameⁱᵐᵖˡ); ("generateNewUIDAndUpdate"%go, State__generateNewUIDAndUpdateⁱᵐᵖˡ); ("objCreate"%go, State__objCreateⁱᵐᵖˡ); ("objDelete"%go, State__objDeleteⁱᵐᵖˡ); ("objGet"%go, State__objGetⁱᵐᵖˡ); ("objList"%go, State__objListⁱᵐᵖˡ); ("objListBySelector"%go, State__objListBySelectorⁱᵐᵖˡ); ("objListLocked"%go, State__objListLockedⁱᵐᵖˡ); ("objUpdate"%go, State__objUpdateⁱᵐᵖˡ)]); (KKey.id, []); (ptrT.id KKey.id, [])].
 
 #[global] Instance info' : PkgInfo apimodel.apimodel :=
   {|
