src/proof/index.v
@@ -1,16 +1,38 @@
 From New.proof Require Import prelude empty_ffi.
-From New.proof Require Export apimodel.
+From New.proof Require Export apimodel list.
+From New.proof.kubernetes_model Require Export apimodel_init.
 
 Section proof.
-Context `{hG: !heapGS Σ} {go_ctx: GoContext}.
-Context `{!mapG Σ KKey.t interface.t}.
 Context `{!mapG Σ KKey.t PureKObject.t}.
 Context `{!mapG Σ KKey.t (gset KKey.t)}.
 Context `{!auth_setG Σ KKey.t}.
+Context `{hG: !heapGS Σ} {go_ctx: GoContext}.
 
-(* TODO: revisit this spec *)
+Lemma wp_index_of_podController index_name obj ptr pod pure_pod dq:
+  {{{ is_pkg_init apimodel ∗
+      "%Hindex_name" ∷ ⌜ index_name = "podController"%go ⌝ ∗
+      "%Hobj" ∷ ⌜ obj = interface.mk (ptrT.id v1.Pod.id) #ptr ⌝ ∗
+      "Hptr" ∷ ptr ↦{dq} pod ∗
+      "Hdeepown_pod" ∷ PurePod.deepown pod pure_pod dq ∗
+      "%Hwell_formed" ∷ ⌜ PurePod.well_formed pure_pod ⌝
+  }}}
+    @! apimodel.index_of #index_name #obj
+  {{{ sl idx_val_list idx_val, RET (#sl, #interface.nil);
+      sl ↦* idx_val_list ∗
+      ⌜ idx_val_list = [idx_val] ⌝ ∗
+      ⌜ ∀ parent_kind parent_name parent_uid,
+        obj_has_controller_parent_of (PureKObject.Pod pure_pod) parent_kind parent_name parent_uid ↔
+        idx_val = pure_pod.(PurePod.ObjectMeta').(PureObjectMeta.Namespace') ++ "/"%go ++
+                  parent_kind ++ "/"%go ++ parent_name ++ "/"%go ++ parent_uid ⌝ ∗
+      ⌜ idx_val = pure_pod.(PurePod.ObjectMeta').(PureObjectMeta.Namespace') ∨ (* the orphan case *)
+        ∃ suffix, idx_val = pure_pod.(PurePod.ObjectMeta').(PureObjectMeta.Namespace') ++ "/"%go ++ suffix ⌝ ∗
+      ptr ↦{dq} pod ∗
+      PurePod.deepown pod pure_pod dq
+  }}}.
+Proof. Admitted.
+
 Lemma wp_State__ByIndex_pod γ l kind index_name indexed_value
-  parent_key owned_parent pod_map owned_child_keys:
+  parent_key owned_parent pure_pod_map owned_child_keys:
   {{{ is_pkg_init apimodel ∗
       "#Hisk" ∷ is_kubernetes γ l ∗
       "%Hkind" ∷ ⌜ kind = "Pod"%go ⌝ ∗
@@ -20,27 +42,200 @@ Lemma wp_State__ByIndex_pod γ l kind index_name indexed_value
                                             parent_key.(KKey.Name') ++ "/"%go ++
                                             (PureKObject.metadata owned_parent).(PureObjectMeta.UID') ⌝ ∗
       "Hown_parent" ∷ parent_key [[ γ.(γ_state) ]]↦ owned_parent ∗
-      "Hown_pod_list" ∷ ([∗ map] key ↦ pod ∈ pod_map, key [[ γ.(γ_state) ]]↦ PureKObject.Pod pod) ∗
+      "Hown_pod_list" ∷ ([∗ map] key ↦ pod ∈ pure_pod_map, key [[ γ.(γ_state) ]]↦ PureKObject.Pod pod) ∗
       "Hown_child_keys" ∷ parent_key [[ γ.(γ_children) ]]↦ owned_child_keys ∗
-      "%Hdom_eq" ∷ ⌜ owned_child_keys = dom pod_map ⌝
+      "%Hdom_eq" ∷ ⌜ owned_child_keys = dom pure_pod_map ⌝
   }}}
     l @ (ptrT.id apimodel.State.id) @ "ByIndex" #kind #index_name #indexed_value
   {{{ objs_l (ptr_list: list loc) (pod_list: list v1.Pod.t) (pure_pod_list: list PurePod.t) dq, RET (#objs_l, #interface.nil);
-      "Hobjs_l" ∷ objs_l ↦* map (λ ptr, interface.mk (ptrT.id v1.Pod.id) #ptr) ptr_list∗
+      "Hobjs_l" ∷ objs_l ↦* map (λ ptr, interface.mk (ptrT.id v1.Pod.id) #ptr) ptr_list ∗
       "Hptrs_pods" ∷ ([∗ list] ptr;pod ∈ ptr_list;pod_list, ptr ↦{dq} pod) ∗
       "Hpods_purepods" ∷ ([∗ list] pod;pure_pod ∈ pod_list;pure_pod_list, PurePod.deepown pod pure_pod dq) ∗
       "%Hwell_formed_pure_pod_list" ∷ ⌜ ∀ p, p ∈ pure_pod_list → PurePod.well_formed p ⌝ ∗
-      "%Hlen_size_eq" ∷ ⌜ length pure_pod_list = size pod_map ⌝ ∗
-      "%Hlist_in_map" ∷  ⌜ ∀ p, p ∈ pure_pod_list → pod_map !! (PurePod.key p) = Some p ⌝ ∗
-      "%Hmap_in_list" ∷ ⌜ ∀ k p, pod_map !! k = Some p → p ∈ pure_pod_list ⌝ ∗
-      "%Hown_pod_keys_eq" ∷ ⌜ ∀ key pod, pod_map !! key = Some pod → key = PurePod.key pod ⌝ ∗
-      "%Hown_pod_list_namespace_eq" ∷ ⌜ ∀ key, key ∈ dom pod_map → key.(KKey.Namespace') = parent_key.(KKey.Namespace') ⌝ ∗
+      "%Hlen_size_eq" ∷ ⌜ length pure_pod_list = size pure_pod_map ⌝ ∗
+      "%Hlist_in_map" ∷  ⌜ ∀ p, p ∈ pure_pod_list → pure_pod_map !! (PurePod.key p) = Some p ⌝ ∗
+      "%Hmap_in_list" ∷ ⌜ ∀ k p, pure_pod_map !! k = Some p → p ∈ pure_pod_list ⌝ ∗
+      "%Hown_pod_keys_eq" ∷ ⌜ ∀ key pod, pure_pod_map !! key = Some pod → key = PurePod.key pod ⌝ ∗
+      "%Hown_pod_list_namespace_eq" ∷ ⌜ ∀ key, key ∈ dom pure_pod_map → key.(KKey.Namespace') = parent_key.(KKey.Namespace') ⌝ ∗
       "%Hno_dup" ∷ ⌜ ∀ i j p1 p2, i ≠ j → pure_pod_list !! i = Some p1 → pure_pod_list !! j = Some p2 → (PurePod.key p1) ≠ (PurePod.key p2) ⌝ ∗
       "Hown_parent" ∷ parent_key [[ γ.(γ_state) ]]↦ owned_parent ∗
-      "Hown_pod_list" ∷ ([∗ map] key ↦ pod ∈ pod_map, key [[ γ.(γ_state) ]]↦ PureKObject.Pod pod) ∗
+      "Hown_pod_list" ∷ ([∗ map] key ↦ pod ∈ pure_pod_map, key [[ γ.(γ_state) ]]↦ PureKObject.Pod pod) ∗
       "Hown_child_keys" ∷ parent_key [[ γ.(γ_children) ]]↦ owned_child_keys
   }}}.
 Proof.
+  wp_start as "H". iNamed "H". iNamed "Hisk".
+  wp_apply wp_with_defer. iIntros (defer) "Hdefer". simpl subst. wp_auto.
+  wp_apply wp_Mutex__Lock; [done|]. iIntros "[Hown_Mutex H]". iNamedPrefix "H" "Hinv_".
+  iAssert (⌜ abs_state !! parent_key = Some (owned_parent) ⌝%I) as "%Hlookup_abs_parent".
+  { iDestruct (map_valid with "Hinv_Hown_abs Hown_parent") as %Hlookup. iPureIntro; exact Hlookup. }
+  iAssert (⌜ children !! parent_key = Some (owned_child_keys) ⌝%I) as "%Hlookup_children".
+  { iDestruct (map_valid with "Hinv_Hown_children Hown_child_keys") as %Hlookup. iPureIntro; exact Hlookup. }
+  wp_auto.
+  wp_apply (wp_State__objListLocked_pod with "[$Hown_pod_list $Hinv_Hstate_m_addr $Hinv_Hown_phys $Hinv_Hown_abs $Hinv_Hphys_abs_rep]").
+  { iPureIntro. split; [done|]. destruct Hinv_Hghost_well_formed. done. }
+  iIntros (sl ptr_list pod_list pure_pod_list) "(Hsl & Hptr_pod_list & Hpod_pure_pod_list & %Hwell_formed & %Hlookup_abs
+    & %Hns_match & %Hmap_in_list & Hinv_Hstate_m_addr & Hinv_Hown_phys & Hinv_Hown_abs & Hinv_Hphys_abs_rep & Hown_pod_list)". wp_auto.
+  assert (∀ (k : KKey.t) (p : PurePod.t), pure_pod_map !! k = Some p → p ∈ pure_pod_list) as Hns_match'.
+  { intros k p Hlookup. apply (Hmap_in_list k p Hlookup). unfold namespace_matches. left. done. }
+  clear Hns_match. rename Hns_match' into Hns_match.
+  set obj_list := map (λ ptr : loc, interface.mk (ptrT.id v1.Pod.id) (# ptr)) ptr_list.
+  assert (length obj_list = length ptr_list) as Hlen_obj_ptr.
+  { unfold obj_list. rewrite map_length. done. }
+  iPoseProof own_slice_nil as "Hslice_nil".
+  iPoseProof own_slice_cap_nil as "Hown_slice_nil_cap".
+  iDestruct (own_slice_len with "Hsl") as %(Hsl_len1 & Hsl_len2).
+  iDestruct (own_slice_wf with "Hsl") as %Hsl_cap.
+  iDestruct (big_sepL2_length with "Hptr_pod_list") as %Hlen_ptr_pod.
+  iDestruct (big_sepL2_length with "Hpod_pure_pod_list") as %Hlen_pod_pure_pod.
+  set P := (λ p, obj_has_controller_parent_of (PureKObject.Pod p) parent_key.(KKey.Kind') parent_key.(KKey.Name') (PureKObject.metadata owned_parent).(PureObjectMeta.UID')).
+  set I := (∃ (i: w64) (val: interface.t) (sl': slice.t) (ptr_list': list loc) (pod_list': list v1.Pod.t) (pure_pod_list': list PurePod.t),
+    "Hi_ptr" ∷ i_ptr ↦ i ∗
+    "Hval_ptr" ∷ val_ptr ↦ val ∗
+    "Hitems_ptr" ∷ items_ptr ↦ sl' ∗
+    "Hsl'" ∷ sl' ↦* map (λ ptr : loc, interface.mk (ptrT.id v1.Pod.id) (# ptr)) ptr_list' ∗
+    "Hptr_pod_list_pre" ∷ ([∗ list] ptr;pod ∈ ptr_list';pod_list', ptr ↦ pod) ∗
+    "Hptr_pod_list_post" ∷ ([∗ list] ptr;pod ∈ (drop (sint.nat i) ptr_list);(drop (sint.nat i) pod_list), ptr ↦ pod) ∗
+    "Hpod_pure_pod_list_pre" ∷ ([∗ list] pod;pure_pod ∈ pod_list';pure_pod_list', PurePod.deepown pod pure_pod 1) ∗
+    "Hpod_pure_pod_list_post" ∷ ([∗ list] pod;pure_pod ∈ (drop (sint.nat i) pod_list);(drop (sint.nat i) pure_pod_list), PurePod.deepown pod pure_pod 1) ∗
+    "Hcap_sl'" :: own_slice_cap interface.t sl' (DfracOwn 1) ∗
+    "%Hfilter_ptr_list" ∷ ⌜ pure_pod_list' = filter P (take (sint.nat i) pure_pod_list) ⌝ ∗
+    "%Hi" ∷ ⌜ 0 ≤ sint.Z i ≤ sint.Z (slice.len_f sl) ⌝
+  )%I.
+  iAssert (I) with "[i val items Hptr_pod_list Hpod_pure_pod_list]" as "Hloop_inv". {
+    iExists (W64 0), (default_val interface.t), (default_val slice.t), [], [], [].
+    iFrame. iFrame "#". rewrite !big_sepL2_nil. done. }
+  wp_for "Hloop_inv". wp_if_destruct.
+  - wp_pure; first word.
+    list_elem obj_list (sint.Z i) as this_obj.
+    wp_apply (wp_load_slice_elem with "[$Hsl]"); [word|eauto| ]. iIntros "Hsl". wp_auto.
+    assert (∃ this_ptr, ptr_list !! sint.nat i = Some this_ptr) as [this_ptr Hthis_ptr_lookup].
+    { apply lookup_lt_is_Some_2. word. }
+    assert (∃ this_pod, pod_list !! sint.nat i = Some this_pod) as [this_pod Hthis_pod_lookup].
+    { apply lookup_lt_is_Some_2. word. }
+    assert (∃ this_pure_pod, pure_pod_list !! sint.nat i = Some this_pure_pod) as [this_pure_pod Hthis_pure_pod_lookup].
+    { apply lookup_lt_is_Some_2. word. }
+    iPoseProof (big_sepL2_destruct_cons _ _ _ this_ptr this_pod with "Hptr_pod_list_post") as "[Hthis_ptr Hother_ptr_pod]".
+    { split. all: rewrite lookup_drop Nat.add_0_r; done. }
+    iPoseProof (big_sepL2_destruct_cons _ _ _ this_pod this_pure_pod with "Hpod_pure_pod_list_post") as "[Hdeepown_this_pod Hother_pod_pure_pod]".
+    { split. all: rewrite lookup_drop Nat.add_0_r; done. }
+    wp_apply (wp_index_of_podController with "[$Hthis_ptr $Hdeepown_this_pod]").
+    { iPureIntro. split_and!; [done| | ].
+      - unfold obj_list in Hthis_obj_lookup. rewrite list_lookup_fmap in Hthis_obj_lookup.
+        rewrite Hthis_ptr_lookup in Hthis_obj_lookup. simpl in Hthis_obj_lookup.
+        injection Hthis_obj_lookup. done.
+      - apply Hwell_formed. apply (list_elem_of_lookup_2 _ (sint.nat i)). done. }
+    iIntros (sl0 idx_val_list idx_val) "(Hsl0 & -> & %Hidx_val & %Hidx_val_prefix & Hthis_ptr & Hdeepown_this_pod)". wp_auto.
+    specialize Hidx_val with parent_key.(KKey.Kind') parent_key.(KKey.Name') (PureKObject.metadata owned_parent).(PureObjectMeta.UID').
+    rewrite bool_decide_true //. wp_auto.
+    wp_alloc j_ptr as "Hj_ptr". wp_auto.
+    iDestruct (own_slice_len with "Hsl0") as %(Hsl0_len1 & _). simpl in Hsl0_len1.
+    set I0 := (∃ (j: w64) (v: go_string) (sl': slice.t),
+      "Hj_ptr" ∷ j_ptr ↦ j ∗
+      "Hv_ptr" ∷ v_ptr ↦ v ∗
+      "Hitems_ptr" ∷ items_ptr ↦ sl' ∗
+      "Hsl'" ∷ sl' ↦* map (λ ptr : loc, interface.mk (ptrT.id v1.Pod.id) (# ptr)) ptr_list' ∗
+      "Hcap_sl'" :: own_slice_cap interface.t sl' (DfracOwn 1) ∗
+      "%Hneg_P" ∷ ⌜ sint.Z j = sint.Z (slice.len_f sl0) → ¬ P this_pure_pod ⌝ ∗
+      "%Hj" ∷ ⌜ 0 ≤ sint.Z j ≤ sint.Z (slice.len_f sl0) ⌝
+    )%I.
+    iAssert (I0) with "[Hj_ptr v Hitems_ptr Hsl' Hcap_sl']" as "Hloop_inv0". {
+      iExists (W64 0), (default_val go_string), sl'.
+      iFrame. iPureIntro. simpl. word. }
+    wp_for "Hloop_inv0". wp_if_destruct.
+    + wp_pure; first word.
+      wp_apply (wp_load_slice_elem with "[$Hsl0]"); [word| | ].
+      { iPureIntro. assert (sint.nat j = 0%nat) as -> by word. done. }
+      iIntros "Hsl0". wp_auto.
+      assert (P this_pure_pod ↔ idx_val = PureObjectMeta.Namespace' (PurePod.ObjectMeta' this_pure_pod) ++ "/"%go ++
+                                          parent_key.(KKey.Kind') ++ "/"%go ++
+                                          parent_key.(KKey.Name') ++ "/"%go ++
+                                          (PureKObject.metadata owned_parent).(PureObjectMeta.UID')) as Hidx_val'.
+      { unfold P. apply Hidx_val. }
+      simpl in Hidx_val'.
+      destruct (bool_decide(P this_pure_pod)) eqn:HP.
+      * apply bool_decide_eq_true in HP.
+        assert (this_pure_pod.(PurePod.ObjectMeta').(PureObjectMeta.Namespace') = parent_key.(KKey.Namespace')) as Hns_eq.
+        { destruct Hinv_Hghost_well_formed. 
+          assert (this_pure_pod.(PurePod.ObjectMeta').(PureObjectMeta.Namespace') = (PurePod.key this_pure_pod).(KKey.Namespace')) as -> by done.
+          symmetry.
+          apply (Hparents_children_same_namespace _ (dom pure_pod_map) _ Hlookup_children).
+          pose proof (split_children_point_to_parent _ _ Hchildren_point_to_parent) as [Hchildren_point_to_parent1 Hchildren_point_to_parent2].
+          assert (abs_state !! PurePod.key this_pure_pod = Some (PureKObject.Pod this_pure_pod)) as Hlookup_abs'.
+          { apply Hlookup_abs. apply (list_elem_of_lookup_2 _ (sint.nat i)). done. }
+          apply (Hchildren_point_to_parent1 parent_key owned_parent (PurePod.key this_pure_pod) (PureKObject.Pod this_pure_pod)).
+          all: try done. }
+        rewrite bool_decide_true //.
+        { rewrite <-Hns_eq. apply Hidx_val'. done. }
+        wp_auto.
+        wp_apply wp_slice_literal. iIntros (sl1) "Hsl1". wp_auto.
+        wp_apply (wp_slice_append with "[$Hsl' $Hcap_sl' $Hsl1]").
+        iIntros (sl'') "(Hsl'' & Hcap_sl'' & Hsl1)". wp_auto.
+        wp_for_post.
+        wp_for_post.
+        iAssert (I) with "[Hi_ptr Hval_ptr Hitems_ptr Hsl'' Hptr_pod_list_pre Hthis_ptr Hother_ptr_pod
+          Hpod_pure_pod_list_pre Hdeepown_this_pod Hother_pod_pure_pod Hcap_sl'']" as "Hloop_inv".
+        { iExists (word.add i (W64 1)), this_obj, sl'', (ptr_list' ++ [this_ptr]), (pod_list' ++ [this_pod]), ((filter P (take (sint.nat i) pure_pod_list)) ++ [this_pure_pod]).
+          assert (map (λ ptr : loc, interface.mk (ptrT.id v1.Pod.id) (# ptr)) ptr_list' ++ [this_obj] =
+                  map (λ ptr, interface.mk (ptrT.id v1.Pod.id) (# ptr)) (ptr_list' ++ [this_ptr])) as ->.
+          { rewrite map_app. simpl.
+            unfold obj_list in Hthis_obj_lookup.
+            rewrite list_lookup_fmap in Hthis_obj_lookup.
+            rewrite Hthis_ptr_lookup in Hthis_obj_lookup.
+            simpl in Hthis_obj_lookup.
+            injection Hthis_obj_lookup as <-.
+            reflexivity. }
+          iFrame.
+          rewrite !big_sepL2_nil.
+          assert (sint.nat (word.add i (W64 1)) = S (sint.nat i)) as -> by word.
+          rewrite !drop_drop Nat.add_1_r.
+          iFrame. iPureIntro. split; [|word].
+          rewrite (take_S_r _ _ this_pure_pod Hthis_pure_pod_lookup).
+          rewrite filter_app. f_equal. unfold filter. simpl.
+          destruct (decide (P this_pure_pod)); [done|done].
+        }
+        iFrame.
+      * apply bool_decide_eq_false in HP.
+        rewrite bool_decide_false //.
+        { destruct (bool_decide(this_pure_pod.(PurePod.ObjectMeta').(PureObjectMeta.Namespace') = parent_key.(KKey.Namespace'))) eqn:Hns.
+          -- apply bool_decide_eq_true in Hns. rewrite <-Hns. intros Heq. apply HP. apply Hidx_val'. done.
+          -- destruct Hidx_val_prefix as [Hidx_val_prefix|Hidx_val_prefix].
+            ++ admit.
+            ++ admit. }
+        wp_auto.
+        wp_for_post.
+        iAssert (I0) with "[Hj_ptr Hv_ptr Hitems_ptr Hsl' Hcap_sl']" as "Hloop_inv0".
+        { iExists (word.add j (W64 1)), idx_val, sl'0. iFrame. iPureIntro. split;[|word]. intros. done. }
+        iFrame.
+    + wp_for_post.
+      iAssert (I) with "[Hi_ptr Hval_ptr Hitems_ptr Hsl' Hptr_pod_list_pre Hthis_ptr Hother_ptr_pod
+        Hpod_pure_pod_list_pre Hdeepown_this_pod Hother_pod_pure_pod Hcap_sl']" as "Hloop_inv".
+      { iExists (word.add i (W64 1)), this_obj, sl'0, ptr_list', pod_list', (filter P (take (sint.nat i) pure_pod_list)).
+        iFrame.
+        assert (sint.nat (word.add i (W64 1)) = S (sint.nat i)) as -> by word.
+        rewrite !drop_drop Nat.add_1_r.
+        iFrame. iPureIntro. split; [|word].
+        rewrite (take_S_r _ _ this_pure_pod Hthis_pure_pod_lookup).
+        rewrite filter_app. unfold filter. simpl.
+        assert (¬ P this_pure_pod) as Hnot_P.
+        { apply Hneg_P. word. }
+        destruct (decide (P this_pure_pod)); [done|].
+        rewrite filter_nil app_nil_r. done. }
+      iFrame.
+  - iCombineNamed "Hinv_*" as "H".
+    wp_apply (wp_Mutex__Unlock _ (kubernetes_inv γ l) with "[$Hown_Mutex H]").
+    { iNamed "H". iFrame. iFrame "#". done. }
+    iApply "HΦ". iFrame "Hsl' Hptr_pod_list_pre Hpod_pure_pod_list_pre". iFrame.
+    iPureIntro.
+    assert ((take (sint.nat i) pure_pod_list) = pure_pod_list) as ->.
+    { apply take_ge. word. }
+    split_and!.
+    * intros p Hpin. apply Hwell_formed. apply list_elem_of_filter in Hpin. destruct Hpin as [_ Hpin]. done.
+    * admit.
+    * admit.
+    * admit.
+    * admit.
+    * admit.
+    * admit. 
 Admitted.
 
 End proof.
